prove process_packet_process'

examples/bloomfilter/main_theorem.v
@@ -1,22 +1,118 @@
 Require Import Poulet4.P4defs.
 Require Import Poulet4.P4Notations.
 Require Import Coq.Program.Basics.
-Open Scope string_scope.
-
-Import ListNotations.
+Require Import Poulet4.Maps.
 Require Import ProD3.examples.bloomfilter.p4ast.
 Require Import ProD3.examples.bloomfilter.bloomfilter.
 Require Import ProD3.examples.bloomfilter.switch.
 Require Import ProD3.examples.bloomfilter.verif.
 
-Require Import Coq.ZArith.ZArith. 
+Require Import Coq.micromega.Lia.
+Require Import Coq.ZArith.ZArith.
 Require Import Coq.Lists.List.
 Import ListNotations.
+Open Scope list_scope.
+Open Scope string_scope.
 
 Require Import ProD3.core.Coqlib.
 
-Print port.
-Definition packet1: BinNums.Z * port := (Z0, port_int).
+Definition process' (bf : bloomfilter_state) (p : Z * port) :=
+  let (data, pt) := p in
+  match pt with
+  | port_int =>
+      (bloomfilter.add Z Z.eqb CRC_pad0 CRC_pad1 CRC_pad2 bf data, (Some (data, port_ext)))
+  | port_ext =>
+      if bloomfilter.query Z CRC_pad0 CRC_pad1 CRC_pad2 bf data then
+        (bf, Some (data, port_int))
+      else
+        (bf, None)
+  end.
+
+Definition bf_encode (es : V1Model.extern_state) (bf : bloomfilter_state) :=
+  PathMap.get ["bloom0"] es = Some (reg_encode (bloom0 bf))
+    /\ PathMap.get ["bloom1"] es = Some (reg_encode (bloom1 bf))
+    /\ PathMap.get ["bloom2"] es = Some (reg_encode (bloom2 bf)).
+
+Open Scope Z_scope.
+
+Lemma sval_refine_to_loptbool_eq : forall w n1 n2,
+  0 <= n1 < Z.pow 2 (Z.of_N w) ->
+  0 <= n2 < Z.pow 2 (Z.of_N w) ->
+  SvalRefine.sval_refine
+    (Value.ValBaseBit (P4Arith.to_loptbool w n1))
+    (Value.ValBaseBit (P4Arith.to_loptbool w n2)) ->
+  n1 = n2.
+Proof.
+Admitted.
+
+Lemma process_packet_prop : forall es bf p es' p',
+  process_packet ge custom_metadata_t es p es' p' ->
+  bf_encode es bf ->
+  exists bf',
+    process' bf p = (bf', p') /\ bf_encode es' bf'.
+Proof.
+  intros.
+  inv H.
+  inv H1. inv H2.
+  eapply (proj1 bloomfilter_body (port_to_Z in_port) data bf) in H6.
+  2 : {
+    clear H5.
+    split. {
+      simpl. unfold AssertionLang.arg_denote, AssertionLang.arg_satisfies.
+      destruct in_port; Tactics.Forall2_sval_refine.
+    }
+    split. {
+      repeat constructor.
+    }
+    destruct H0 as [? []].
+    repeat constructor.
+    - red; simpl; destruct (PathMap.get ["bloom0"] es); inv H; auto.
+    - red; simpl; destruct (PathMap.get ["bloom1"] es); inv H0; auto.
+    - red; simpl; destruct (PathMap.get ["bloom2"] es); inv H1; auto.
+  }
+  destruct H6 as  [? [? []]].
+  exists (fst (process (port_to_Z in_port) data bf)).
+  split.
+  2 : {
+    destruct H6 as [? [? []]].
+    repeat constructor.
+    - red in H6; simpl in H6; destruct (PathMap.get ["bloom0"] es'); inv H6; auto.
+    - red in H7; simpl in H7; destruct (PathMap.get ["bloom1"] es'); inv H7; auto.
+    - red in H8; simpl in H8; destruct (PathMap.get ["bloom2"] es'); inv H8; auto.
+  }
+  assert (data' = data
+    /\ out_port_to_Z out_port = snd (process (port_to_Z in_port) data bf)).
+  {
+    inv H.
+    split.
+    - clear -H3 H4 H10.
+      subst hdr'.
+      inv H10. inv H1. destruct H5.
+      clear -H3 H4 H0. inv H0. inv H7. destruct H2.
+      clear -H3 H4 H0.
+      apply sval_refine_to_loptbool_eq in H0; eauto.
+    - inv H12. inv H13.
+      clear -H5 H11.
+      apply SvalRefine.sval_refine_get with (f := "egress_spec") in H11.
+      simpl in H11.
+      rewrite H5 in H11.
+      apply sval_refine_to_loptbool_eq in H11; eauto.
+      + destruct in_port; simpl.
+        2 : destruct (query Z CRC_pad0 CRC_pad1 CRC_pad2 bf data); simpl.
+        all : lia.
+      + destruct out_port as [[] | ]; simpl.
+        all : lia.
+  }
+  clear -H7.
+  destruct H7; subst.
+  unfold process, process' in *.
+  destruct in_port; destruct out_port as [[] | ];
+    simpl in *; try solve [inv H0]; auto;
+    destruct (query Z CRC_pad0 CRC_pad1 CRC_pad2 bf data);
+    try solve [inv H0]; auto.
+Qed.
+
+(* Definition packet1: BinNums.Z * port := (Z0, port_int).
 Definition packet2: BinNums.Z * port := (1%Z, port_ext).
 
 Lemma Test1: forall st' output,
@@ -85,12 +181,12 @@ subst inst_path.
 inv H2.
 apply H in H10.
 specialize (H  bloomfilter_state
-apply H in H10. simpl in H.  in H10.*)
+apply H in H10. simpl in H.  in H10.
 Check (FuncSpec.fundef_satisfies_spec _ _ tgt ge bloomfilter_spec).
 bloomfilter_spec.
 
-Check bloomfilter_body. *)Search FuncSpec.fundef_satisfies_spec Semantics.exec_func .
+Check bloomfilter_body. Search FuncSpec.fundef_satisfies_spec Semantics.exec_func .
 Print FuncSpec.fundef_satisfies_spec_aux.
 Print FuncSpec.fundef_satisfies_hoare.
 Search Semantics.exec_func.
-inversion H3. simpl in *.
+inversion H3. simpl in *. *)
