examples/bloomfilter/switch.v
@@ -44,27 +44,34 @@ Inductive port :=
   | port_int
   | port_ext.
 
-Definition port_to_sval (p : port) :=
+Definition port_to_Z (p : port) :=
   match p with
-  | port_int => ValBaseBit (P4Arith.to_loptbool 9 0)
-  | port_ext => ValBaseBit (P4Arith.to_loptbool 9 1)
+  | port_int => 0
+  | port_ext => 1
+  end.
+
+Definition port_to_sval (p : port) :=
+  ValBaseBit (P4Arith.to_loptbool 9 (port_to_Z p)).
+
+Definition out_port_to_Z (p : option port) :=
+  match p with
+  | Some p => port_to_Z p
+  | None => 511
   end.
 
 Definition out_port_to_sval (p : option port) :=
-  match p with
-  | Some p => port_to_sval p
-  | None => ValBaseBit (P4Arith.to_loptbool 9 511)
-  end.
+  ValBaseBit (P4Arith.to_loptbool 9 (out_port_to_Z p)).
 
 Inductive process_packet : extern_state -> (Z * port) -> extern_state -> option (Z * port) -> Prop :=
   | process_packet_intro : forall es data in_port es' data' out_port meta' std_meta' class_name inst_path fd m',
       PathMap.get ["main"; "ig"] (ge_inst ge) = Some {|iclass:=class_name; ipath:=inst_path|} ->
       PathMap.get ([class_name; "apply"]) (ge_func ge) = Some fd ->
-      0 <= data < (Z.pow 2 16 - 1) ->
+      0 <= data < Z.pow 2 16 ->
       let hdr := ValBaseStruct [("myHeader",
         ValBaseHeader [("data", ValBaseBit (P4Arith.to_loptbool 16 data))] (Some true))] in
       let meta := force ValBaseNull (uninit_sval_of_typ None M) in
       let std_meta := update "ingress_port" (port_to_sval in_port) (force ValBaseNull (uninit_sval_of_typ None standard_metadata_t)) in
+      0 <= data' < Z.pow 2 16 ->
       let hdr' := ValBaseStruct [("myHeader",
         ValBaseHeader [("data", ValBaseBit (P4Arith.to_loptbool 16 data'))] (Some true))] in
       Members.get "egress_spec" std_meta' = out_port_to_sval out_port ->
